src/progress.lean
@@ -1,3 +1,4 @@
+/-
 import .syntax .notations .logic .evaluation .vcgen .bindings
 
 @[reducible]
@@ -261,3 +262,5 @@ theorem progress {s: stack} {Q: propctx}: (⊢ₛ s : Q) → is_value s ∨ ∃s
       )
     }
   end
+
+-/
