README.md
@@ -4,3 +4,4 @@ This repository contains a formal definition of [esverify](https://esverify.org/
 and proves properties such as verification safety and type translation correctness.
 
 The definitions and proofs are written in [LEAN](http://leanprover.github.io/).
+
